\documentclass[a4paper,12pt]{article}
\usepackage{amsmath}

\begin{document}

\section*{Laplace Transform of Derivatives}

\subsection*{Example:}
Given that $ L\{F(t)\} = f(s) $, then show that:
\[
L\{F'(t)\} = sf(s) - F(0).
\]

\subsection*{Solution:}
Given that $ L\{F(t)\} = f(s) $ \quad ... (1)

By the definition of the Laplace transform, we get:
\[
L\{F'(t)\} = \int_{0}^{\infty} e^{-st} F'(t) \, dt.
\]

Using integration by parts:
\[
L\{F'(t)\} = \left[ e^{-st} F(t) \right]_{0}^{\infty} + s \int_{0}^{\infty} e^{-st} F(t) \, dt.
\]

Since $ e^{-\infty} = 0 $:
\[
L\{F'(t)\} = 0 - e^{0} F(0) + s \int_{0}^{\infty} e^{-st} F(t) \, dt,
\]
\[
L\{F'(t)\} = -F(0) + s f(s). \quad \text{(Using equation (1))}
\]

Thus:
\[
L\{F'(t)\} = sf(s) - F(0). \quad \text{(Proved)}
\]

\subsection*{Key Equations:}

\subsection*{First-Order Derivative:}
The Laplace transform of the first derivative is given by:
\[
L\{F'(t)\} = s f(s) - F(0).
\]

\subsection*{Second-Order Derivative:}
The Laplace transform of the second derivative is given by:
\[
L\{F''(t)\} = s^2 f(s) - s F(0) - F'(0).
\]

\subsection*{Third-Order Derivative:}
The Laplace transform of the third derivative is given by:
\[
L\{F^{(3)}(t)\} = s^3 f(s) - s^2 F(0) - s F'(0) - F''(0).
\]

\subsection*{$n$-th Order Derivative:}
The Laplace transform of the $n$-th derivative is given by:
\[
L\{F^{(n)}(t)\} = s^n f(s) - s^{n-1} F(0) - s^{n-2} F'(0) - \dots - s F^{(n-2)}(0) - F^{(n-1)}(0).
\]

\section*{Laplace Transform of a Function Divided by $t$}

\textbf{Example:} If $ L\{F(t)\} = f(s) $, then:
\[
L\left\{\frac{F(t)}{t}\right\} = \int_s^\infty f(u) \, du.
\]


\section*{Laplace Transform of Integrals}

\textbf{Example:} If $ L\{F(t)\} = f(s) $, then:
\begin{enumerate}
    \item
    \[
    L\left\{\int_0^t F(u) \, du\right\} = \frac{f(s)}{s}.
    \]

    \item
    \[
    L\left\{\int_0^t \frac{\sin u}{u} \, du\right\} = \frac{1}{s} \tan^{-1}\frac{1}{s}.
    \]
\end{enumerate}

\end{document}
